Prove propositional state decoding correct

Base.thy
@@ -21,6 +21,17 @@ proof -
     then show ?case by blast
   qed
 qed
-
 end
+
+definition restr_set::"(nat \<Rightarrow> 't) \<Rightarrow> nat \<Rightarrow> 't set" where
+"restr_set f n = f ` {..<n}"
+
+lemma restr_set_bij: "bij_betw f {..<n} S \<Longrightarrow> restr_set f n = S"
+  apply (subst restr_set_def)
+  apply (subst (asm) bij_betw_def)
+  by (drule conjunct2)
+
+lemma lt_in_restr: "n < m \<Longrightarrow> f n \<in> restr_set f m"
+  using restr_set_def by fast
+
 end
