Diagonal_Timed_Automata.thy
@@ -169,4 +169,10 @@ where
 
 declare steps.intros[intro]
 
+lemma steps_trans: "A \<turnstile> \<langle>l, u\<rangle> \<rightarrow>* \<langle>l', u'\<rangle> \<Longrightarrow> A \<turnstile> \<langle>l', u'\<rangle> \<rightarrow>* \<langle>l'', u''\<rangle> \<Longrightarrow> A \<turnstile> \<langle>l, u\<rangle> \<rightarrow>* \<langle>l'', u''\<rangle>"
+  by (induction rule: steps.induct) auto
+
+lemma steps_twist: "A \<turnstile> \<langle>l, u\<rangle> \<rightarrow>* \<langle>l', u'\<rangle> \<Longrightarrow> A \<turnstile> \<langle>l', u'\<rangle> \<rightarrow> \<langle>l'', u''\<rangle> \<Longrightarrow> A \<turnstile> \<langle>l, u\<rangle> \<rightarrow>* \<langle>l'', u''\<rangle>"
+  by (induction rule: steps.induct) auto
+
 end
